src/program_proof/session/nat_equivalence.v
@@ -7,6 +7,10 @@ Class Similarity (A : Type) (B : Type) : Type :=
 
 Infix "=~=" := is_similar_to.
 
+#[global]
+Instance Similarity_prod {A : Type} {A' : Type} {B : Type} {B' : Type} (A_SIM : Similarity A A') (B_SIM : Similarity B B') : Similarity (A * B) (A' * B') :=
+  fun p : A * B => fun p' : A' * B' => p.1 =~= p'.1 /\ p.2 =~= p'.2.
+
 Inductive list_corres {A : Type} {B : Type} {SIM : Similarity A B} : Similarity (list A) (list B) :=
   | nil_corres
     : [] =~= []
@@ -16,9 +20,510 @@ Inductive list_corres {A : Type} {B : Type} {SIM : Similarity A B} : Similarity 
     : x :: xs =~= y :: ys.
 
 #[global]
-Instance Similarity_list_list {A : Type} {B : Type} (SIM : Similarity A B) : Similarity (list A) (list B) :=
+Instance Similarity_list {A : Type} {B : Type} (SIM : Similarity A B) : Similarity (list A) (list B) :=
   @list_corres A B SIM.
 
+Lemma Similarity_list_length {A : Type} {B : Type} {SIM : Similarity A B} (xs : list A) (ys : list B)
+  (H_sim : xs =~= ys)
+  : length xs = length ys.
+Proof.
+  induction H_sim as [ | ? ? ? ? ? ? IH]; simpl; congruence.
+Qed.
+
+Definition UPPER_BOUND : Z :=
+  2 ^ 64.
+
 #[global]
-Instance Similarity_u64_nat : Similarity u64 nat :=
-  fun x => fun y => (y = uint.nat x)%nat /\ (uint.Z x >= 0 /\ uint.Z x < 2 ^ 64)%Z.
+Instance Similarity_u64 : Similarity u64 nat :=
+  fun u => fun n => (n = uint.nat u)%nat /\ (uint.Z u >= 0 /\ uint.Z u < UPPER_BOUND)%Z.
+
+Lemma Similarity_u64_range (u : u64) (n : nat)
+  (H_sim : u =~= n)
+  : (uint.Z u >= 0 /\ uint.Z u < UPPER_BOUND)%Z.
+Proof.
+  do 2 red in H_sim. word.
+Qed.
+
+Module Operation'.
+
+  Record t : Set :=
+    mk
+    { VersionVector : list nat
+    ; Data : nat
+    }.
+
+  Record corres (op : Operation.t) (op' : Operation'.t) : Prop :=
+    Similarity_Operation_INTRO
+    { VersionVector_corres : op.(Operation.VersionVector) =~= op'.(VersionVector)
+    ; Data_corres : op.(Operation.Data) =~= op'.(Data)
+    }.
+
+End Operation'.
+
+#[global]
+Instance Similarity_Operation : Similarity Operation.t Operation'.t :=
+  Operation'.corres.
+
+Module Message'.
+
+  Record t : Set :=
+    mk
+    { MessageType : nat
+    ; C2S_Client_Id : nat
+    ; C2S_Server_Id : nat
+    ; C2S_Client_OperationType : nat
+    ; C2S_Client_Data : nat
+    ; C2S_Client_VersionVector : list nat
+    ; S2S_Gossip_Sending_ServerId : nat
+    ; S2S_Gossip_Receiving_ServerId : nat
+    ; S2S_Gossip_Operations : list Operation'.t
+    ; S2S_Gossip_Index : nat
+    ; S2S_Acknowledge_Gossip_Sending_ServerId : nat
+    ; S2S_Acknowledge_Gossip_Receiving_ServerId : nat
+    ; S2S_Acknowledge_Gossip_Index : nat
+    ; S2C_Client_OperationType : nat
+    ; S2C_Client_Data : nat
+    ; S2C_Client_VersionVector : list nat
+    ; S2C_Server_Id : nat
+    ; S2C_Client_Number : nat
+    }.
+
+  Record corres (msg : Message.t) (msg' : Message'.t) : Prop :=
+    Similarity_Message_INTRO
+    { MessageType_corres : msg.(Message.MessageType) =~= msg'.(MessageType)
+    ; C2S_Client_Id_corres : msg.(Message.C2S_Client_Id) =~= msg'.(C2S_Client_Id)
+    ; C2S_Server_Id_corres : msg.(Message.C2S_Server_Id) =~= msg'.(C2S_Server_Id)
+    ; C2S_Client_OperationType_corres : msg.(Message.C2S_Client_OperationType) =~= msg'.(C2S_Client_OperationType)
+    ; C2S_Client_Data_corres_corres : msg.(Message.C2S_Client_Data) =~= msg'.(C2S_Client_Data)
+    ; C2S_Client_VersionVector_corres : msg.(Message.C2S_Client_VersionVector) =~= msg'.(C2S_Client_VersionVector)
+    ; S2S_Gossip_Sending_ServerId_corres : msg.(Message.S2S_Gossip_Sending_ServerId) =~= msg'.(S2S_Gossip_Sending_ServerId)
+    ; S2S_Gossip_Receiving_ServerId_corres : msg.(Message.S2S_Gossip_Receiving_ServerId) =~= msg'.(S2S_Gossip_Receiving_ServerId)
+    ; S2S_Gossip_Operations_corres : msg.(Message.S2S_Gossip_Operations) =~= msg'.(S2S_Gossip_Operations)
+    ; S2S_Gossip_Index_corres : msg.(Message.S2S_Gossip_Index) =~= msg'.(S2S_Gossip_Index)
+    ; S2S_Acknowledge_Gossip_Sending_ServerId_corres : msg.(Message.S2S_Acknowledge_Gossip_Sending_ServerId) =~= msg'.(S2S_Acknowledge_Gossip_Sending_ServerId)
+    ; S2S_Acknowledge_Gossip_Receiving_ServerId_corres : msg.(Message.S2S_Acknowledge_Gossip_Receiving_ServerId) =~= msg'.(S2S_Acknowledge_Gossip_Receiving_ServerId)
+    ; S2S_Acknowledge_Gossip_Index_corres : msg.(Message.S2S_Acknowledge_Gossip_Index) =~= msg'.(S2S_Acknowledge_Gossip_Index)
+    ; S2C_Client_OperationType_corres : msg.(Message.S2C_Client_OperationType) =~= msg'.(S2C_Client_OperationType)
+    ; S2C_Client_Data_corres : msg.(Message.S2C_Client_Data) =~= msg'.(S2C_Client_Data)
+    ; S2C_Client_VersionVector_corres : msg.(Message.S2C_Client_VersionVector) =~= msg'.(S2C_Client_VersionVector)
+    ; S2C_Server_Id_corres : msg.(Message.S2C_Server_Id) =~= msg'.(S2C_Server_Id)
+    ; S2C_Client_Number_corres : msg.(Message.S2C_Client_Number) =~= msg'.(S2C_Client_Number)
+    }.
+
+End Message'.
+
+#[global]
+Instance Similarity_Message : Similarity Message.t Message'.t :=
+  Message'.corres.
+
+Module Server'.
+
+  Record t : Set :=
+    mk
+    { Id : nat
+    ; NumberOfServers : nat
+    ; UnsatisfiedRequests : list Message'.t
+    ; VectorClock : list nat
+    ; OperationsPerformed : list Operation'.t
+    ; MyOperations : list Operation'.t
+    ; PendingOperations : list Operation'.t
+    ; GossipAcknowledgements : list nat
+    }.
+
+  Record corres (server : Server.t) (server' : Server'.t) : Prop :=
+    Similarity_Server_INTRO
+    { Id_corres : server.(Server.Id) =~= server'.(Id)
+    ; NumberOfServers_corres : server.(Server.NumberOfServers) =~= server'.(NumberOfServers)
+    ; UnsatisfiedRequests_corres : server.(Server.UnsatisfiedRequests) =~= server'.(UnsatisfiedRequests)
+    ; VectorClock_corres : server.(Server.VectorClock) =~= server'.(VectorClock)
+    ; OperationsPerformed_corres : server.(Server.OperationsPerformed) =~= server'.(OperationsPerformed)
+    ; MyOperations_corres : server.(Server.MyOperations) =~= server'.(MyOperations)
+    ; PendingOperations_corres : server.(Server.PendingOperations) =~= server'.(PendingOperations)
+    ; GossipAcknowledgements_corres : server.(Server.GossipAcknowledgements) =~= server'.(GossipAcknowledgements)
+    }.
+
+End Server'.
+
+#[global]
+Instance Similarity_Server : Similarity Server.t Server'.t :=
+  Server'.corres.
+
+Module Client'.
+
+  Record t : Set :=
+    mk
+    { Id : nat
+    ; NumberOfServers : nat
+    ; WriteVersionVector : list nat
+    ; ReadVersionVector : list nat
+    ; SessionSemantic : nat
+    }.
+
+  Record corres (client : Client.t) (client' : Client'.t) : Prop :=
+    Similarity_Client_INTRO
+    { Id_corres : client.(Client.Id) =~= client'.(Id)
+    ; NumberOfServers_corres : client.(Client.NumberOfServers) =~= client'.(NumberOfServers)
+    ; WriteVersionVector_corres : client.(Client.WriteVersionVector) =~= client'.(WriteVersionVector)
+    ; ReadVersionVector_corres : client.(Client.ReadVersionVector) =~= client'.(ReadVersionVector)
+    ; SessionSemantic_corres : client.(Client.SessionSemantic) =~= client'.(SessionSemantic)
+    }.
+
+End Client'.
+
+#[global]
+Instance Similarity_Client : Similarity Client.t Client'.t :=
+  Client'.corres.
+
+Module NatImplServer.
+
+  Fixpoint coq_compareVersionVector (v1 : list nat) (v2 : list nat) : bool :=
+    match v1 with
+    | [] => true
+    | h1 :: t1 =>
+      match v2 with
+      | [] => true
+      | h2 :: t2 => negb (h1 <? h2)%nat && coq_compareVersionVector t1 t2
+      end
+    end.
+
+  Fixpoint coq_lexicographicCompare (v1 : list nat) (v2 : list nat) : bool :=
+    match v1 with
+    | [] => false 
+    | h1 :: t1 =>
+      match v2 with
+      | [] => false 
+      | h2 :: t2 => if (h1 =? h2)%nat then coq_lexicographicCompare t1 t2 else (h1 >? h2)%nat
+      end
+    end.
+
+  Definition coq_maxTwoInts (x : nat) (y : nat) : nat :=
+    if (x >? y)%nat then x else y. 
+
+  Fixpoint coq_maxTS (v1 : list nat) (v2 : list nat) : list nat :=
+    match v1 with
+    | [] => []
+    | h1 :: t1 =>
+      match v2 with
+      | [] => [] 
+      | h2 :: t2 => coq_maxTwoInts h1 h2 :: coq_maxTS t1 t2
+      end
+    end.
+
+  Definition coq_oneOffVersionVector (v1 : list nat) (v2 : list nat) : bool :=
+    let loop_init : bool * bool :=
+      (true, true)
+    in
+    let loop_step (acc : bool * bool) (element : nat * nat) : bool * bool :=
+      let (e1, e2) := element in
+      let (output, canApply) := acc in
+      if canApply && (e1 + 1 =? e2)%nat then
+        (output, false)
+      else if (e1 >=? e2)%nat then
+        (output, canApply)
+      else 
+        (false, canApply)
+    in
+    let (output, canApply) := fold_left loop_step (zip v1 v2) loop_init in
+    output && negb canApply.
+
+  Fixpoint coq_equalSlices (s1 : list nat) (s2 : list nat) : bool :=
+    match s1 with
+    | [] => true
+    | h1 :: t1 => 
+      match s2 with
+      | [] => true
+      | h2 :: t2 => (h1 =? h2)%nat && coq_equalSlices t1 t2
+      end
+    end.
+
+  Definition coq_equalOperations (o1 : Operation'.t) (o2 : Operation'.t) : bool :=
+    coq_equalSlices o1.(Operation'.VersionVector) o2.(Operation'.VersionVector) && (o1.(Operation'.Data) =? o2.(Operation'.Data))%nat.
+
+  Fixpoint coq_sortedInsert (l : list Operation'.t) (i : Operation'.t) : list Operation'.t :=
+    match l with
+    | [] => [i]
+    | h :: t =>
+      if orb (coq_lexicographicCompare h.(Operation'.VersionVector) i.(Operation'.VersionVector)) (coq_equalSlices h.(Operation'.VersionVector) i.(Operation'.VersionVector))
+      then (i :: h :: t)%list
+      else (h :: coq_sortedInsert t i)%list
+    end.
+
+  Definition coq_mergeOperations (l1 : list Operation'.t) (l2 : list Operation'.t) : list Operation'.t :=
+    let output := fold_left coq_sortedInsert l2 l1 in
+    let loop_init : nat * list Operation'.t :=
+      (0%nat, [])
+    in
+    let loop_step (acc : nat * list Operation'.t) (element : Operation'.t) : nat * list Operation'.t :=
+      let (index, acc) := acc in
+      match (output !! (index + 1)%nat) with
+      | Some v => if (coq_equalOperations element v) then ((index + 1)%nat, acc) else ((index + 1)%nat, acc ++ [element])
+      | None => ((index + 1)%nat, acc ++ [element])
+      end
+    in
+    snd (fold_left loop_step output loop_init).
+
+  Definition coq_deleteAtIndexOperation (o : list Operation'.t) (index : nat) : list Operation'.t :=
+    take index o ++ drop (index + 1) o.
+
+  Definition coq_deleteAtIndexMessage (m : list Message'.t) (index : nat) : list Message'.t :=
+    take index m ++ drop (index + 1) m.
+
+  Definition coq_getDataFromOperationLog (l : list Operation'.t) : nat :=
+    match l !! (length l - 1)%nat with
+    | Some v => v.(Operation'.Data)
+    | None => 0%nat
+    end.
+
+  Definition coq_receiveGossip (s : Server'.t) (r : Message'.t) : Server'.t :=
+    if (length r.(Message'.S2S_Gossip_Operations) =? 0)%nat then
+      s
+    else
+      let focus := coq_mergeOperations s.(Server'.PendingOperations) r.(Message'.S2S_Gossip_Operations) in
+      let loop_init : nat * Server'.t :=
+        (0%nat, Server'.mk s.(Server'.Id) s.(Server'.NumberOfServers) s.(Server'.UnsatisfiedRequests) s.(Server'.VectorClock) s.(Server'.OperationsPerformed) s.(Server'.MyOperations) focus s.(Server'.GossipAcknowledgements))
+      in
+      let loop_step (acc : nat * Server'.t) (e : Operation'.t) : nat * Server'.t :=
+        let '(i, s) := acc in
+        if coq_oneOffVersionVector s.(Server'.VectorClock) e.(Operation'.VersionVector) then
+          let OperationsPerformed := coq_mergeOperations s.(Server'.OperationsPerformed) [e] in
+          let VectorClock := coq_maxTS s.(Server'.VectorClock) e.(Operation'.VersionVector) in
+          let PendingOperations := coq_deleteAtIndexOperation s.(Server'.PendingOperations) i in
+          (i, Server'.mk s.(Server'.Id) s.(Server'.NumberOfServers) s.(Server'.UnsatisfiedRequests) VectorClock OperationsPerformed s.(Server'.MyOperations) PendingOperations s.(Server'.GossipAcknowledgements))
+        else ((i + 1)%nat, s)
+      in
+      snd (fold_left loop_step focus loop_init).
+
+  Definition coq_acknowledgeGossip (s : Server'.t) (r : Message'.t) : Server'.t :=
+    let i := r.(Message'.S2S_Acknowledge_Gossip_Sending_ServerId) in
+    let l := s.(Server'.GossipAcknowledgements) in
+    if (i >=? length l)%nat then
+      s
+    else
+      let prevGossipAcknowledgementsValue : nat :=
+        match s.(Server'.GossipAcknowledgements) !! i with
+        | Some x => x
+        | None => 0%nat
+        end
+      in
+      let newGossipAcknowledgements := coq_maxTwoInts prevGossipAcknowledgementsValue r.(Message'.S2S_Acknowledge_Gossip_Index) in
+      let gossipAcknowledgements := <[i := newGossipAcknowledgements]> l in
+      Server'.mk s.(Server'.Id) s.(Server'.NumberOfServers) s.(Server'.UnsatisfiedRequests) s.(Server'.VectorClock) s.(Server'.OperationsPerformed) s.(Server'.MyOperations) s.(Server'.PendingOperations) gossipAcknowledgements.
+
+  Definition coq_getGossipOperations (s : Server'.t) (serverId : nat) : list Operation'.t :=
+    match s.(Server'.GossipAcknowledgements) !! serverId with
+    | Some v => drop v s.(Server'.MyOperations)
+    | None => []
+    end.
+
+  Definition coq_processClientRequest (s : Server'.t) (r : Message'.t) : bool * Server'.t * Message'.t :=
+    if negb (coq_compareVersionVector s.(Server'.VectorClock) r.(Message'.C2S_Client_VersionVector)) then
+      (false, s, (Message'.mk 0 0 0 0 0 [] 0 0 [] 0 0 0 0 0 0 [] 0 0))
+    else
+      if (r.(Message'.C2S_Client_OperationType) =? 0)%nat then
+        let S2C_Client_Data := coq_getDataFromOperationLog s.(Server'.OperationsPerformed) in
+        let S2C_Client_VersionVector := s.(Server'.VectorClock) in
+        let S2C_Client_Number := r.(Message'.C2S_Client_Id) in
+        let S2C_Server_Id := s.(Server'.Id) in
+        (true, s, (Message'.mk 4 0 0 0 0 [] 0 0 [] 0 0 0 0 0 S2C_Client_Data S2C_Client_VersionVector S2C_Server_Id S2C_Client_Number))
+      else
+        let v := list_lookup_total s.(Server'.Id) s.(Server'.VectorClock) in
+        let VectorClock := <[s.(Server'.Id) := (v + 1)%nat]> s.(Server'.VectorClock) in
+        let OperationsPerformed := coq_sortedInsert s.(Server'.OperationsPerformed) (Operation'.mk VectorClock r.(Message'.C2S_Client_Data)) in
+        let MyOperations := coq_sortedInsert s.(Server'.MyOperations) (Operation'.mk VectorClock r.(Message'.C2S_Client_Data)) in
+        let S2C_Client_OperationType := 1%nat in
+        let S2C_Client_Data := 0%nat in
+        let S2C_Client_VersionVector := VectorClock in
+        let S2C_Client_Number := r.(Message'.C2S_Client_Id) in
+        let S2C_Server_Id := s.(Server'.Id) in
+        (true, Server'.mk s.(Server'.Id) s.(Server'.NumberOfServers) s.(Server'.UnsatisfiedRequests) VectorClock OperationsPerformed MyOperations s.(Server'.PendingOperations) s.(Server'.GossipAcknowledgements), (Message'.mk 4 0 0 0 0 [] 0 0 [] 0 0 0 0 1 S2C_Client_Data S2C_Client_VersionVector S2C_Server_Id S2C_Client_Number)).
+
+  Definition coq_processRequest (server : Server'.t) (request : Message'.t) : Server'.t * list Message'.t :=
+    match request.(Message'.MessageType) with
+    | 0%nat =>
+      let '(succeeded, server, reply) := coq_processClientRequest server request in
+      if succeeded then
+        (server, [reply])
+      else
+        let UnsatisfiedRequests := server.(Server'.UnsatisfiedRequests) ++ [request] in 
+        let server := Server'.mk server.(Server'.Id) server.(Server'.NumberOfServers) UnsatisfiedRequests server.(Server'.VectorClock) server.(Server'.OperationsPerformed) server.(Server'.MyOperations) server.(Server'.PendingOperations) server.(Server'.GossipAcknowledgements) in
+        (server, [])
+    | 1%nat =>
+      let server := coq_receiveGossip server request in
+      let focus := server.(Server'.UnsatisfiedRequests) in
+      let loop_init : nat * (Server'.t * list Message'.t) :=
+        (0%nat, (server, [Message'.mk 2 0 0 0 0 [] 0 0 [] 0 (server.(Server'.Id)) (request.(Message'.S2S_Gossip_Sending_ServerId)) (request.(Message'.S2S_Gossip_Index)) 0 0 [] 0 0]))
+      in
+      let loop_step (acc : nat * (Server'.t * list Message'.t)) (element : Message'.t) : nat * (Server'.t * list Message'.t) :=
+        let '(i, (s, outGoingRequests)) := acc in
+        let '(succeeded, s, reply) := coq_processClientRequest s element in
+        if succeeded then
+          let UnsatisfiedRequests := coq_deleteAtIndexMessage s.(Server'.UnsatisfiedRequests) i in
+          (i, (Server'.mk s.(Server'.Id) s.(Server'.NumberOfServers) UnsatisfiedRequests s.(Server'.VectorClock) s.(Server'.OperationsPerformed) s.(Server'.MyOperations) s.(Server'.PendingOperations) s.(Server'.GossipAcknowledgements), outGoingRequests ++ [reply]))
+        else
+          ((i + 1)%nat, (s, outGoingRequests))
+      in
+      snd (fold_left loop_step focus loop_init)
+    | 2%nat => (coq_acknowledgeGossip server request, [])
+    | 3%nat =>
+      let loop_init : list Message'.t :=
+        []
+      in
+      let loop_step (acc : list Message'.t) (index : nat) : list Message'.t :=
+        if negb (index =? (server.(Server'.Id)))%nat && negb (length (coq_getGossipOperations server index) =? 0)%nat then
+          let S2S_Gossip_Sending_ServerId := server.(Server'.Id) in
+          let S2S_Gossip_Receiving_ServerId := index in
+          let S2S_Gossip_Operations := coq_getGossipOperations server index in
+          let S2S_Gossip_Index := length server.(Server'.MyOperations) in
+          let message := Message'.mk 1 0 0 0 0 [] S2S_Gossip_Sending_ServerId S2S_Gossip_Receiving_ServerId S2S_Gossip_Operations S2S_Gossip_Index 0 0 0 0 0 [] 0 0 in
+          acc ++ [message]
+        else
+          acc
+      in
+      (server, fold_left loop_step (seq 0%nat (uint.nat server.(Server'.NumberOfServers))) loop_init)
+    | _ => (server, [])
+    end.
+
+  Section EQUIVALENCE.
+
+    #[local]
+    Instance Similarity_bool : Similarity bool bool :=
+      @eq bool.
+
+    #[local]
+    Instance Similarity_fun {D : Type} {D' : Type} {C : Type} {C' : Type} (D_SIM : Similarity D D') (C_SIM : Similarity C C') : Similarity (D -> C) (D' -> C') :=
+      fun f : D -> C => fun f' : D' -> C' => forall x, forall x', x =~= x' -> f x =~= f' x'.
+
+    Lemma coq_compareVersionVector_corres
+      : CoqSessionServer.coq_compareVersionVector =~= coq_compareVersionVector.
+    Admitted.
+  
+    Lemma coq_lexicographicCompare_corres
+      : CoqSessionServer.coq_lexicographicCompare =~= coq_lexicographicCompare.
+    Admitted.
+  
+    Lemma coq_maxTwoInts_corres
+      : CoqSessionServer.coq_maxTwoInts =~= coq_maxTwoInts.
+    Admitted.
+  
+    Lemma coq_maxTS_corres
+      : CoqSessionServer.coq_maxTS =~= coq_maxTS.
+    Admitted.
+  
+    Lemma coq_oneOffVersionVector_corres
+      : CoqSessionServer.coq_oneOffVersionVector =~= coq_oneOffVersionVector.
+    Admitted.
+  
+    Lemma coq_equalSlices_corres
+      : CoqSessionServer.coq_equalSlices =~= coq_equalSlices.
+    Admitted.
+  
+    Lemma coq_equalOperations_corres
+      : CoqSessionServer.coq_equalOperations =~= coq_equalOperations.
+    Admitted.
+  
+    Lemma coq_sortedInsert_corres
+      : CoqSessionServer.coq_sortedInsert =~= coq_sortedInsert.
+    Admitted.
+  
+    Lemma coq_mergeOperations_corres
+      : CoqSessionServer.coq_mergeOperations =~= coq_mergeOperations.
+    Admitted.
+  
+    Lemma coq_deleteAtIndexOperation_corres
+      : CoqSessionServer.coq_deleteAtIndexOperation =~= coq_deleteAtIndexOperation.
+    Admitted.
+  
+    Lemma coq_deleteAtIndexMessage_corres
+      : CoqSessionServer.coq_deleteAtIndexMessage =~= coq_deleteAtIndexMessage.
+    Admitted.
+  
+    Lemma coq_getDataFromOperationLog_corres
+      : CoqSessionServer.coq_getDataFromOperationLog =~= coq_getDataFromOperationLog.
+    Admitted.
+  
+    Lemma coq_receiveGossip_corres
+      : CoqSessionServer.coq_receiveGossip =~= coq_receiveGossip.
+    Admitted.
+  
+    Lemma coq_acknowledgeGossip_corres
+      : CoqSessionServer.coq_acknowledgeGossip =~= coq_acknowledgeGossip.
+    Admitted.
+
+    Lemma coq_getGossipOperations_corres
+      : CoqSessionServer.coq_getGossipOperations =~= coq_getGossipOperations.
+    Admitted.
+
+    Lemma coq_processClientRequest_corres
+      : CoqSessionServer.coq_processClientRequest =~= coq_processClientRequest.
+    Admitted.
+  
+    Lemma coq_processRequest_corres
+      : CoqSessionServer.coq_processRequest =~= coq_processRequest.
+    Admitted.
+
+  End EQUIVALENCE.
+
+End NatImplServer.
+
+Export NatImplServer.
+
+Module NatImplClient.
+
+  Definition coq_read (c : Client'.t) (serverId : nat) : Message'.t :=
+    match c.(Client'.SessionSemantic) with
+    | 0%nat => Message'.mk 0 c.(Client'.Id) serverId 0 0 [] 0 0 [] 0 0 0 0 0 0 [] 0 0
+    | 1%nat => Message'.mk 0 c.(Client'.Id) serverId 0 0 [] 0 0 [] 0 0 0 0 0 0 [] 0 0
+    | 2%nat => Message'.mk 0 c.(Client'.Id) serverId 0 0 [] 0 0 [] 0 0 0 0 0 0 [] 0 0
+    | 3%nat => Message'.mk 0 c.(Client'.Id) serverId 0 0 c.(Client'.ReadVersionVector) 0 0 [] 0 0 0 0 0 0 [] 0 0
+    | 4%nat => Message'.mk 0 c.(Client'.Id) serverId 0 0 c.(Client'.WriteVersionVector) 0 0 [] 0 0 0 0 0 0 [] 0 0
+    | 5%nat => Message'.mk 0 c.(Client'.Id) serverId 0 0 (coq_maxTS c.(Client'.WriteVersionVector) c.(Client'.ReadVersionVector)) 0 0 [] 0 0 0 0 0 0 [] 0 0
+    | _ => Message'.mk 0 0 0 0 0 [] 0 0 [] 0 0 0 0 0 0 [] 0 0
+    end.
+
+  Definition coq_write (c : Client'.t) (serverId : nat) (value : nat) : Message'.t :=
+    match c.(Client'.SessionSemantic) with
+    | 0%nat => Message'.mk 0 c.(Client'.Id) serverId 1 value [] 0 0 [] 0 0 0 0 0 0 [] 0 0
+    | 1%nat => Message'.mk 0 c.(Client'.Id) serverId 1 value c.(Client'.ReadVersionVector) 0 0 [] 0 0 0 0 0 0 [] 0 0
+    | 2%nat => Message'.mk 0 c.(Client'.Id) serverId 1 value c.(Client'.WriteVersionVector) 0 0 [] 0 0 0 0 0 0 [] 0 0
+    | 3%nat => Message'.mk 0 c.(Client'.Id) serverId 1 value [] 0 0 [] 0 0 0 0 0 0 [] 0 0
+    | 4%nat => Message'.mk 0 c.(Client'.Id) serverId 1 value [] 0 0 [] 0 0 0 0 0 0 [] 0 0
+    | 5%nat => Message'.mk 0 c.(Client'.Id) serverId 1 value (coq_maxTS c.(Client'.WriteVersionVector) c.(Client'.ReadVersionVector)) 0 0 [] 0 0 0 0 0 0 [] 0 0
+    | _ => Message'.mk 0 0 0 0 0 [] 0 0 [] 0 0 0 0 0 0 [] 0 0
+    end.
+
+  Definition coq_processRequest (c : Client'.t) (requestType : nat) (serverId : nat) (value : nat) (ackMessage : Message'.t) : Client'.t * Message'.t :=
+    match requestType with
+    | 0%nat => (c, coq_read c serverId)
+    | 1%nat => (c, coq_write c serverId value)
+    | 2%nat =>
+      match ackMessage.(Message'.S2C_Client_OperationType) with
+      | 0%nat => (Client'.mk c.(Client'.Id) c.(Client'.NumberOfServers) c.(Client'.WriteVersionVector) ackMessage.(Message'.S2C_Client_VersionVector) c.(Client'.SessionSemantic), Message'.mk 0 0 0 0 0 [] 0 0 [] 0 0 0 0 0 0 [] 0 0)
+      | 1%nat => (Client'.mk c.(Client'.Id) c.(Client'.NumberOfServers) (ackMessage.(Message'.S2C_Client_VersionVector)) c.(Client'.ReadVersionVector) c.(Client'.SessionSemantic), Message'.mk 0 0 0 0 0 [] 0 0 [] 0 0 0 0 0 0 [] 0 0)
+      | _ => (c, Message'.mk 0 0 0 0 0 [] 0 0 [] 0 0 0 0 0 0 [] 0 0)
+      end
+    | _ => (c, Message'.mk 0 0 0 0 0 [] 0 0 [] 0 0 0 0 0 0 [] 0 0)
+    end.
+
+  Section EQUIVALENCE.
+
+    #[local] Existing Instance Similarity_bool.
+
+    #[local] Existing Instance Similarity_fun.
+
+    Lemma coq_read_corres
+      : CoqSessionClient.coq_read =~= coq_read.
+    Admitted.
+
+    Lemma coq_write_corres
+      : CoqSessionClient.coq_write =~= coq_write.
+    Admitted.
+  
+    Lemma coq_processRequest_corres
+      : CoqSessionClient.coq_processRequest =~= coq_processRequest.
+    Admitted.
+
+  End EQUIVALENCE.
+
+End NatImplClient.
+
+Export NatImplClient.
